generic/Zeta.Generic.TSLog.fsti
@@ -24,10 +24,10 @@ val lemma_prefix_clock_sorted (#vspec #n:_) (itsl: its_log vspec n) (i:nat{i <= 
   Lemma (ensures (clock_sorted (prefix itsl i)))
         [SMTPat (prefix itsl i)]
 
-val create (#vspec:_) (gl: G.verifiable_log vspec): (itsl:its_log vspec (S.length gl){to_glog itsl == gl})
+val create (#vspec:_) (gl: G.verifiable_log vspec): GTot (itsl:its_log vspec (S.length gl){to_glog itsl == gl})
 
 val prefix_within_epoch (#vspec #n:_) (ep: epoch) (itsl: its_log vspec n)
-  : itsl': its_log vspec n {itsl' `SA.prefix_of` itsl}
+  : GTot (itsl': its_log vspec n {itsl' `SA.prefix_of` itsl})
 
 val prefix_within_epoch_correct (#vspec #n:_) (ep: epoch) (itsl: its_log vspec n) (i: seq_index itsl)
   : Lemma (ensures (let il' = prefix_within_epoch ep itsl in
